low/Extraction.v
@@ -16,6 +16,14 @@ Set Extraction AccessOpaque.
    (otherwise, useless errors will be launched). *)
 Extraction Inline (*epsilon epsilon_def*) classicT arbitrary indefinite_description (*Inhab_witness*) Fix isTrue.
 
+Extract Constant default_input =>
+  "let string_to_char_list str =
+     let rec aux i acc =
+       if i < 0 then acc
+       else aux (i - 1) (str.[i] :: acc) in
+     aux (String.length str - 1) [] in {
+   prompt_string = (let rec t _ = lazy (Stream_intro (string_to_char_list (input_line stdin), t ())) in t ()) ;
+   random_boolean = (let rec t _ = lazy (Stream_intro (Random.bool (), t ())) in t ()) }".
 
 Extract Inductive positive => "int"
 [ "(fun p -> 1 + (2 * p))"
